ramified function specs allow us to call functions without
creating an evar for the frame, but instead implicitly instantiate
the frame with
(wand calleePost callerPost)
which can be thought of as
"callerPost minus calleePost"

which solves the problem that variables introduced during cancellation
are not in the evar context of the frame evar.

bedrock2/src/bedrock2/HeapletwiseHyps.v
@@ -25,6 +25,52 @@ Section HeapletwiseHyps.
   Context {key value: Type} {mem: map.map key value} {mem_ok: map.ok mem}
           {key_eqb: key -> key -> bool} {key_eqb_spec: EqDecider key_eqb}.
 
+  Lemma split_du: forall (m m1 m2: mem),
+      map.split m m1 m2 <-> Some m = mmap.du (Some m1) (Some m2).
+  Proof.
+    unfold map.split, mmap.du, map.du. split; intros; fwd.
+    - eapply map.disjointb_spec in Hp1. rewrite Hp1. reflexivity.
+    - eapply map.disjointb_spec in E. auto.
+  Qed.
+
+  (* with mmap.du instead of map.split:
+  Definition wand(P1 P2: mem -> Prop): mem -> Prop :=
+    fun mdiff => forall m1 m2, Some m2 = mmap.du (Some m1) (Some mdiff) -> P1 m1 -> P2 m2. *)
+
+  Definition wand(P1 P2: mem -> Prop): mem -> Prop :=
+    fun mdiff => forall m1 m2, map.split m2 mdiff m1 -> P1 m1 -> P2 m2.
+
+  Lemma wand_adjoint: forall (P Q R: mem -> Prop),
+      impl1 (sep P Q) R <-> impl1 P (wand Q R).
+  Proof.
+    unfold impl1, sep, wand. intros; split; intros; fwd; eauto 7.
+  Qed.
+
+  (* modus ponens for wand only holds in one direction! *)
+  Lemma wand_mp: forall P Q,
+      impl1 (sep P (wand P Q)) Q.
+  Proof.
+    intros. rewrite sep_comm. rewrite (wand_adjoint (wand P Q) P Q). reflexivity.
+  Qed.
+
+  Lemma ramify_funspec_hyp: forall (calleePre calleePost callerPost: mem -> Prop) m,
+      (* non-ramified hypothesis: requires creating an evar for Frame too early *)
+      (exists Frame,
+          sep calleePre Frame m /\ (forall m', sep calleePost Frame m' -> callerPost m')) <->
+      (* ramified hypothesis: no frame needed *)
+      sep calleePre (wand calleePost callerPost) m.
+  Proof.
+    split; intros; fwd.
+    - revert m Hp0.
+      change (impl1 (sep calleePre Frame) (sep calleePre (wand calleePost callerPost))).
+      reify_goal. ecancel_step_by_implication. cbn [seps].
+      eapply (wand_adjoint Frame calleePost callerPost). rewrite sep_comm. unfold impl1.
+      exact Hp1.
+    - eexists. split. 1: exact H.
+      change (impl1 (sep calleePost (wand calleePost callerPost)) callerPost).
+      eapply wand_mp.
+  Qed.
+
   Lemma sep_assoc_eq: forall (p q r: mem -> Prop),
       sep (sep p q) r = sep p (sep q r).
   Proof.
@@ -305,7 +351,16 @@ Section HeapletwiseHypsTests.
     eapply frobenicate_ok.
     split. {
       start_canceling.
-      repeat canceling_step.
+
+      (* if this was splitting memories, instantiating ?R with (eq the-split-memories),
+         we'd get evar scoping problems!
+         -> instantiate with mem predicates instead of eq?
+
+         -> trick like ramified frame rule?
+       *)
+
+      canceling_step.
+      canceling_step.
       eapply canceling_done_frame.
     }
     intros_after_mem_modification.
@@ -323,6 +378,153 @@ Section HeapletwiseHypsTests.
     eapply canceling_done_empty.
   Qed.
 
+  Lemma frobenicate_ok_ramified: forall (a1 a2 v1 v2: nat) (m: mem) (P: mem -> Prop),
+      sep (foo v1 a1) (sep (foo v2 a2) (* <-- calleePre *)
+        (wand (sep (foo (v1 + v2) a1) (foo (v1 - v2) a2)) (* <-- calleePost *)
+              P (* <-- callerPost *))) m ->
+      wp (frobenicate a1 a2) m P.
+  Proof.
+    intros. eapply sep_assoc in H. eapply ramify_funspec_hyp in H. fwd.
+    eapply frobenicate_ok. split.
+    - eapply sep_assoc. eassumption.
+    - rewrite <- sep_assoc_eq. assumption.
+  Qed.
+
+  (* sample caller: *)
+  Goal forall (p1 p2 p3 x y: nat) (m: mem) (R: mem -> Prop),
+      sep (foo x p1) (sep (foo y p2) (sep (foo x p3) R)) m ->
+      wp (frobenicate p1 p3) m (fun m' =>
+        wp (frobenicate p3 p1) m' (fun m'' =>
+           sep (foo 0 p1) (sep (foo y p2) (sep (foo (x + x) p3) R)) m'')).
+  Proof.
+    intros.
+    repeat split_sep_step.
+    repeat merge_du_step.
+    reify_disjointness_hyp.
+
+    eapply frobenicate_ok_ramified. (* <- evars created for arguments, but not for frame! *)
+    start_canceling.
+    canceling_step.
+    canceling_step.
+    unfold wand.
+    unfold canceling.
+    unfold seps.
+    setoid_rewrite split_du.
+    unfold mmap.dus.
+    intros.
+    repeat split_sep_step.
+    repeat merge_du_step.
+    reify_disjointness_hyp.
+    repeat clear_unused_mem_hyps_step.
+    clear m.
+
+    eapply frobenicate_ok_ramified. (* <- evars created for arguments, but not for frame! *)
+    start_canceling.
+    canceling_step.
+    canceling_step.
+    unfold wand.
+    unfold canceling.
+    unfold seps.
+    setoid_rewrite split_du.
+    unfold mmap.dus.
+    intros.
+    repeat split_sep_step.
+    repeat merge_du_step.
+    reify_disjointness_hyp.
+    repeat clear_unused_mem_hyps_step.
+
+    rewrite PeanoNat.Nat.sub_diag in *.
+    rewrite PeanoNat.Nat.add_0_l in *.
+    rewrite PeanoNat.Nat.sub_0_l in *.
+
+    start_canceling.
+    repeat canceling_step.
+    eapply canceling_done_empty.
+  Qed.
+
   Let foo_pair(v1 v2 a1 a2: nat) := sep (foo v1 a1) (foo v2 a2).
+
+  (* sample caller where argument is a field: *)
+  Goal forall (p1 p2 p3 x y: nat) (m: mem) (R: mem -> Prop),
+      sep (foo x p1) (sep (foo_pair y x p2 p3) R) m ->
+      wp (frobenicate p1 p3) m (fun m' =>
+        wp (frobenicate p3 p1) m' (fun m'' =>
+           sep (foo 0 p1) (sep (foo_pair y (x + x) p2 p3) R) m'')).
+  Proof.
+    intros.
+    repeat split_sep_step.
+    repeat merge_du_step.
+    reify_disjointness_hyp.
+
+    eapply frobenicate_ok.
+    split. { (* <-- actually, should not split, but canceling mechanism doesn't support
+      "seps m /\ Rest" format yet, and it might actually not be needed at all *)
+      start_canceling.
+      canceling_step.
+
+      (* need to modify hyps while canceling: *)
+      unfold foo_pair in H2.
+      unfold with_mem in H2.
+      split_sep_step.
+      replace [Some m2; Some m3] with [Some m1; Some m4; Some m3] by admit.
+      (* not literally, but implied by definition of canceling *)
+      clear m2 D.
+
+      (* now we can continue canceling: *)
+      canceling_step.
+
+      assert_fails (eapply canceling_done_frame).
+      (* PROBLEM: Would like to instantiate ?R
+         with (fun m => Some m = mmap.dus (Some m1) (Some m4))
+         but m1 and m4 are not in ?R's scope!
+
+  H0 : m0 |= foo x p1
+  H1 : m1 |= foo y p2
+  H4 : m4 |= foo x p3
+  H3 : m3 |= R
+  ============================
+  canceling [?R] [Some m1; Some m3]     *)
+
+  Abort.
+
+  (* sample caller where argument is a field: *)
+  Goal forall (p1 p2 p3 x y: nat) (m: mem) (R: mem -> Prop),
+      sep (foo x p1) (sep (foo_pair y x p2 p3) R) m ->
+      wp (frobenicate p1 p3) m (fun m' =>
+        wp (frobenicate p3 p1) m' (fun m'' =>
+           sep (foo 0 p1) (sep (foo_pair y (x + x) p2 p3) R) m'')).
+  Proof.
+    intros.
+    repeat split_sep_step.
+    repeat merge_du_step.
+    reify_disjointness_hyp.
+
+    eapply frobenicate_ok_ramified.
+    start_canceling.
+    canceling_step.
+    unfold foo_pair in H2.
+    unfold with_mem in H2.
+    split_sep_step.
+    replace [Some m2; Some m3] with [Some m1; Some m4; Some m3] by admit.
+    (* not literally, but implied by definition of canceling *)
+    clear m2 D.
+    canceling_step.
+    (* here, there's no frame left that we would need to instantiate with
+       (fun m => Some m = mmap.dus (Some m1) (Some m4))
+       which would violate evar scopes because m1 and m4 were introduced after the frame *)
+    unfold wand.
+    unfold canceling.
+    unfold seps.
+    setoid_rewrite split_du.
+    unfold mmap.dus.
+    intros.
+    repeat split_sep_step.
+    repeat merge_du_step.
+    reify_disjointness_hyp.
+    repeat clear_unused_mem_hyps_step.
+    clear m.
+
+    (* rest should work as well *)
+  Abort.
 
 End HeapletwiseHypsTests.
